src/tls/MITLS.Repr.Handshake13.fst
@@ -50,38 +50,38 @@ module NSTRepr  = MITLS.Repr.NewSessionTicket13
 
 type t = HSM13.handshake13
 
-type repr (b:R.slice) =
+type repr (b:R.const_slice) =
   R.repr_p t b HSM13.handshake13_parser
 
-let is_eoed (#b:R.slice) (r:repr b) : GTot bool =
+let is_eoed (#b:R.const_slice) (r:repr b) : GTot bool =
   HSM13.M13_end_of_early_data? (R.value r)
 
-let is_ee (#b:R.slice) (r:repr b) : GTot bool =
+let is_ee (#b:R.const_slice) (r:repr b) : GTot bool =
   HSM13.M13_encrypted_extensions? (R.value r)
 
-let is_cr (#b:R.slice) (r:repr b) : GTot bool =
+let is_cr (#b:R.const_slice) (r:repr b) : GTot bool =
   HSM13.M13_certificate_request? (R.value r)
 
-let is_c (#b:R.slice) (r:repr b) : GTot bool =
+let is_c (#b:R.const_slice) (r:repr b) : GTot bool =
   HSM13.M13_certificate? (R.value r)
 
-let is_cv (#b:R.slice) (r:repr b) : GTot bool =
+let is_cv (#b:R.const_slice) (r:repr b) : GTot bool =
   HSM13.M13_certificate_verify? (R.value r)
 
-let is_fin (#b:R.slice) (r:repr b) : GTot bool =
+let is_fin (#b:R.const_slice) (r:repr b) : GTot bool =
   HSM13.M13_finished? (R.value r)
 
-let is_nst (#b:R.slice) (r:repr b) : GTot bool =
+let is_nst (#b:R.const_slice) (r:repr b) : GTot bool =
   HSM13.M13_new_session_ticket? (R.value r)
 
-let is_kupd (#b:R.slice) (r:repr b) : GTot bool =
+let is_kupd (#b:R.const_slice) (r:repr b) : GTot bool =
   HSM13.M13_key_update? (R.value r)
 
 (*
  * Common precondition for functions that return the
  *   reprs for specific instance types
  *)
-unfold let repr_pre (#b:R.slice) (r:repr b)
+unfold let repr_pre (#b:R.const_slice) (r:repr b)
   : HS.mem -> Type0
   = fun h -> R.valid r h
 
@@ -90,7 +90,7 @@ unfold let repr_pre (#b:R.slice) (r:repr b)
  *   reprs for specific instance types
  *)
 unfold let repr_post_common
-  (#b:R.slice)
+  (#b:R.const_slice)
   (#a:Type) (#k:LP.parser_kind) (#p:LP.parser k a)
   (r:repr b)  //input repr
   : HS.mem -> R.repr_p a b p -> HS.mem -> Type0
@@ -101,21 +101,21 @@ unfold let repr_post_common
     r.start_pos <= rr.start_pos /\  //slice indices for the instance repr are contained in the slice indices of r ...
     rr.end_pos <= r.end_pos  //... useful for framing
 
-let get_ee_repr (#b:R.slice) (r:repr b{is_ee r})
+let get_ee_repr (#b:R.const_slice) (r:repr b{is_ee r})
   : Stack (EERepr.repr b)
     (requires repr_pre r)
     (ensures  fun h0 rr h1 ->
       R.value r == HSM13.M13_encrypted_extensions (R.value rr) /\
       repr_post_common r h0 rr h1)
   = R.reveal_valid ();
+    let lp_b = R.to_slice b in
+    let pos = HSM13.handshake13_accessor_encrypted_extensions lp_b r.R.start_pos in
+    let pos = HSM13.handshake13_m13_encrypted_extensions_accessor lp_b pos in
+    let end_pos = Parsers.EncryptedExtensions.encryptedExtensions_jumper lp_b pos in
 
-    let pos = HSM13.handshake13_accessor_encrypted_extensions b r.R.start_pos in
-    let pos = HSM13.handshake13_m13_encrypted_extensions_accessor b pos in
-    let end_pos = Parsers.EncryptedExtensions.encryptedExtensions_jumper b pos in
+    R.mk_from_const_slice b pos end_pos Parsers.EncryptedExtensions.encryptedExtensions_parser
 
-    R.mk b pos end_pos Parsers.EncryptedExtensions.encryptedExtensions_parser
-
-let get_c_repr (#b:R.slice) (r:repr b{is_c r})
+let get_c_repr (#b:R.const_slice) (r:repr b{is_c r})
   : Stack (CRepr.repr b)
     (requires repr_pre r)
     (ensures  fun h0 rr h1 ->
@@ -124,77 +124,80 @@ let get_c_repr (#b:R.slice) (r:repr b{is_c r})
       R.value r == HSM13.M13_certificate (R.value rr) /\
       repr_post_common r h0 rr h1)
   = R.reveal_valid ();
+    let lp_b = R.to_slice b in
+    let pos = HSM13.handshake13_accessor_certificate lp_b r.R.start_pos in
+    let pos = HSM13.handshake13_m13_certificate_accessor lp_b pos in
+    let end_pos = Parsers.Certificate13.certificate13_jumper lp_b pos in
 
-    let pos = HSM13.handshake13_accessor_certificate b r.R.start_pos in
-    let pos = HSM13.handshake13_m13_certificate_accessor b pos in
-    let end_pos = Parsers.Certificate13.certificate13_jumper b pos in
+    R.mk_from_const_slice b pos end_pos Parsers.Certificate13.certificate13_parser
 
-    R.mk b pos end_pos Parsers.Certificate13.certificate13_parser
-
-let get_cv_repr (#b:R.slice) (r:repr b{is_cv r})
+let get_cv_repr (#b:R.const_slice) (r:repr b{is_cv r})
   : Stack (CVRepr.repr b)
     (requires repr_pre r)
     (ensures  fun h0 rr h1 ->
       R.value r = HSM13.M13_certificate_verify (R.value rr) /\
       repr_post_common r h0 rr h1)
   = R.reveal_valid ();
+    let lp_b = R.to_slice b in
+    let pos = HSM13.handshake13_accessor_certificate_verify lp_b r.R.start_pos in
+    let pos = HSM13.handshake13_m13_certificate_verify_accessor lp_b pos in
+    let end_pos = Parsers.CertificateVerify13.certificateVerify13_jumper lp_b pos in
 
-    let pos = HSM13.handshake13_accessor_certificate_verify b r.R.start_pos in
-    let pos = HSM13.handshake13_m13_certificate_verify_accessor b pos in
-    let end_pos = Parsers.CertificateVerify13.certificateVerify13_jumper b pos in
+    R.mk_from_const_slice b pos end_pos Parsers.CertificateVerify13.certificateVerify13_parser
 
-    R.mk b pos end_pos Parsers.CertificateVerify13.certificateVerify13_parser
-
-let get_fin_repr (#b:R.slice) (r:repr b{is_fin r})
+let get_fin_repr (#b:R.const_slice) (r:repr b{is_fin r})
   : Stack (FinRepr.repr b)
     (requires repr_pre r)
     (ensures  fun h0 rr h1 ->
       R.value r == HSM13.M13_finished (R.value rr) /\
       repr_post_common r h0 rr h1)
   = R.reveal_valid ();
+    let lp_b = R.to_slice b in
+    let pos = HSM13.handshake13_accessor_finished lp_b r.R.start_pos in
+    let end_pos = HSM13.handshake13_m13_finished_jumper lp_b pos in
 
-    let pos = HSM13.handshake13_accessor_finished b r.R.start_pos in
-    let end_pos = HSM13.handshake13_m13_finished_jumper b pos in
+    R.mk_from_const_slice b pos end_pos HSM13.handshake13_m13_finished_parser
 
-    R.mk b pos end_pos HSM13.handshake13_m13_finished_parser
-
-let get_cr_repr (#b:R.slice) (r:repr b{is_cr r})
+let get_cr_repr (#b:R.const_slice) (r:repr b{is_cr r})
   : Stack (CRRepr.repr b)
     (requires repr_pre r)
     (ensures  fun h0 rr h1 ->
       R.value r == HSM13.M13_certificate_request (R.value rr) /\
       repr_post_common r h0 rr h1)
   = R.reveal_valid ();
+    let lp_b = R.to_slice b in
 
-    let pos = HSM13.handshake13_accessor_certificate_request b r.R.start_pos in
-    let pos = HSM13.handshake13_m13_certificate_request_accessor b pos in
-    let end_pos = Parsers.CertificateRequest13.certificateRequest13_jumper b pos in
+    let pos = HSM13.handshake13_accessor_certificate_request lp_b r.R.start_pos in
+    let pos = HSM13.handshake13_m13_certificate_request_accessor lp_b pos in
+    let end_pos = Parsers.CertificateRequest13.certificateRequest13_jumper lp_b pos in
 
-    R.mk b pos end_pos Parsers.CertificateRequest13.certificateRequest13_parser
+    R.mk_from_const_slice b pos end_pos Parsers.CertificateRequest13.certificateRequest13_parser
 
-let get_eoed_repr (#b:R.slice) (r:repr b{is_eoed r})
+let get_eoed_repr (#b:R.const_slice) (r:repr b{is_eoed r})
   : Stack (EoEDRepr.repr b)
     (requires repr_pre r)
     (ensures  fun h0 rr h1 ->
       R.value r == HSM13.M13_end_of_early_data (R.value rr) /\
       repr_post_common r h0 rr h1)
   = R.reveal_valid ();
+    let lp_b = R.to_slice b in
 
-    let pos = HSM13.handshake13_accessor_end_of_early_data b r.R.start_pos in
-    let end_pos = HSM13.handshake13_m13_end_of_early_data_jumper b pos in
+    let pos = HSM13.handshake13_accessor_end_of_early_data lp_b r.R.start_pos in
+    let end_pos = HSM13.handshake13_m13_end_of_early_data_jumper lp_b pos in
 
-    R.mk b pos end_pos HSM13.handshake13_m13_end_of_early_data_parser
+    R.mk_from_const_slice b pos end_pos HSM13.handshake13_m13_end_of_early_data_parser
 
-let get_nst_repr (#b:R.slice) (r:repr b{is_nst r})
+let get_nst_repr (#b:R.const_slice) (r:repr b{is_nst r})
   : Stack (NSTRepr.repr b)
     (requires repr_pre r)
     (ensures  fun h0 rr h1 ->
       R.value r == HSM13.M13_new_session_ticket (R.value rr) /\
       repr_post_common r h0 rr h1)
   = R.reveal_valid ();
+    let lp_b = R.to_slice b in
 
-    let pos = HSM13.handshake13_accessor_new_session_ticket b r.R.start_pos in
-    let pos = HSM13.handshake13_m13_new_session_ticket_accessor b pos in
-    let end_pos = Parsers.NewSessionTicket13.newSessionTicket13_jumper b pos in
+    let pos = HSM13.handshake13_accessor_new_session_ticket lp_b r.R.start_pos in
+    let pos = HSM13.handshake13_m13_new_session_ticket_accessor lp_b pos in
+    let end_pos = Parsers.NewSessionTicket13.newSessionTicket13_jumper lp_b pos in
 
-    R.mk b pos end_pos Parsers.NewSessionTicket13.newSessionTicket13_parser
+    R.mk_from_const_slice b pos end_pos Parsers.NewSessionTicket13.newSessionTicket13_parser
